\begin{quote}
	\textbf{Proposition}
Suppose the fluid is in the region $D$ and $x\in D$. Let $\textbf{y} = \textbf{x} + \textbf{h}$ be a nearby point, then
\begin{equation}
\textbf{u}(\textbf{y},t) = \textbf{u}(\textbf{x},t) + \textbf{D}(\textbf{x},t)\cdot \textbf{h} + \frac{1}{2}\mathbf{\xi}(\textbf{x},t)\cdot \textbf{h} + \mathcal{O}\left(\lVert \textbf{h}\rVert^2\right),
\end{equation}
where $\textbf{D}(\textbf{x},t)$ is a symmetric $3\times 3$ matrix, $\textbf{h}=(h_1,h_2,h_3)$ and $\textbf{u}=(u_1,u_2,u_3)$.
\end{quote}

\paragraph{proof} % H5 title

Note that
\begin{equation}
\nabla \textbf{u} = \left(\frac{\partial u_i}{\partial x_j}\right)_{1\leq i,j\leq 3}
= \begin{pmatrix}
\frac{\partial u_1}{\partial x_1} & \frac{\partial u_1}{\partial x_2} & \frac{\partial u_1}{\partial x_3}\\
\frac{\partial u_2}{\partial x_1} & \frac{\partial u_2}{\partial x_2} & \frac{\partial u_2}{\partial x_3}\\
\frac{\partial u_3}{\partial x_1} & \frac{\partial u_3}{\partial x_2} & \frac{\partial u_3}{\partial x_3}
\end{pmatrix}
\end{equation}
and 
\begin{equation}
\begin{aligned}
u_i(\textbf{y},t) - u_i(\textbf{x},t)
&= u_i(\textbf{x}+\textbf{h},t) - u_i(\textbf{x},t)\\
&= \int_{0}^{1}\frac{\partial}{\partial s} u_i(\textbf{x}+s\textbf{h},t)ds,
\quad\text{let $\textbf{z}=\textbf{x}+s\textbf{h}$}\\
&=  \int_{0}^{1} \sum_{j=1}^{3} \frac{\partial u_i(\textbf{z},t)}{\partial z_j}\frac{\partial z_j}{\partial s}ds\\
&= \sum_{j=1}^{3} \int_{0}^{1} \frac{\partial}{\partial z_j}u_i(\textbf{x}+s\textbf{h},t)h_j\,ds\\
&= \sum_{j=1}^{3}\int_{0}^{1} \left(\frac{\partial}{\partial z_j}u_i(\textbf{x}+s\textbf{h},t) + \frac{\partial}{\partial x_j}u_i(\textbf{x},t) - \frac{\partial}{\partial x_j}u_i(\textbf{x},t)\right)h_j\,ds\\
&= \sum_{j=1}^{3}\int_{0}^{1}\frac{\partial}{\partial x_j}u_i(\textbf{x},t)ds + \sum_{j=1}^{3}\int_{0}^{1} \left(\frac{\partial}{\partial z_j}u_i(\textbf{x}+s\textbf{h},t)  - \frac{\partial}{\partial x_j}u_i(\textbf{x},t)\right)h_j\,ds\\
&= \sum_{j=1}^{3}\frac{\partial}{\partial x_j}u_i(\textbf{x},t)
+ \sum_{j=1}^{3}\int_{0}^{1} h_j \left(\frac{\partial}{\partial z_j}u_i(\textbf{x}+s\textbf{h},t)  - \frac{\partial}{\partial x_j}u_i(\textbf{x},t)\right)\,ds\\
&= \sum_{j=1}^{3}\frac{\partial}{\partial x_j}u_i(\textbf{x},t)
+ \sum_{j=1}^{3}\int_{0}^{1} h_j \left(\int_{0}^{1}\frac{\partial}{\partial s'}
\left(\frac{\partial}{\partial z_j}u_i(\textbf{x}+s's\textbf{h},t)\right) ds'\right)\,ds,
\quad\text{let $\textbf{w}=\textbf{x}+s's\textbf{h}$}\\
&= \sum_{j=1}^{3}\frac{\partial}{\partial x_j}u_i(\textbf{x},t)
+ \sum_{j=1}^{3}\int_{0}^{1} h_j \left(\int_{0}^{1}\sum_{m=1}^{3}\frac{\partial}{\partial w_m}\left(\frac{\partial}{\partial z_j}u_i(\textbf{x}+s's\textbf{h},t)\right)\frac{\partial w_m}{\partial s'}ds'\right)\,ds\\
&= \sum_{j=1}^{3}\frac{\partial}{\partial x_j}u_i(\textbf{x},t)
+ \sum_{j,m=1}^{3}\int_{0}^{1} h_j \left(\int_{0}^{1}\frac{\partial}{\partial w_m}\frac{\partial}{\partial z_j}u_i(\textbf{x}+s's\textbf{h},t)(sh_m)ds'\right)\,ds\\
&= \sum_{j=1}^{3}\frac{\partial}{\partial x_j}u_i(\textbf{x},t)
+ \sum_{j,m=1}^{3} h_j h_m \int_{0}^{1}\int_{0}^{1}s\frac{\partial^2}{\partial w_m \partial z_j}u_i(\textbf{x}+s's\textbf{h},t)ds'\,ds\\
&= \sum_{j=1}^{3}\frac{\partial}{\partial x_j}u_i(\textbf{x},t)
+ \sum_{j,m=1}^{3} h_j h_m \int_{0}^{1}\int_{0}^{1}s\frac{\partial^2}{\partial x_m \partial x_j}u_i(\textbf{x}+s's\textbf{h},t)ds'\,ds\\
\end{aligned}
\end{equation}
Then we let
\begin{equation}
\left\{\begin{aligned}
E
&= \sum_{j,m=1}^{3} h_j h_m \int_{0}^{1}\int_{0}^{1}s\frac{\partial^2}{\partial x_m \partial x_j}u_i(\textbf{x}+s's\textbf{h},t)ds'\,ds\\
C_{j,m}
&= \int_{0}^{1}\int_{0}^{1}s\frac{\partial^2}{\partial x_m \partial x_j}u_i(\textbf{x}+s's\textbf{h},t)ds'\,ds
\end{aligned}\right.
\end{equation}



consider
\begin{equation}
\abs{E} \leq \sum_{j,m=1}^{3} C_{j,m}\abs{h_j}\abs{h_m}\leq C'\lVert \textbf{h}\rVert^2
\end{equation}
we have
\begin{equation}
u_i(\textbf{y},t) = u_i(\textbf{x},t) + \sum_{j=1}^{3}\frac{\partial}{\partial x_j}u_{i}(\textbf{x},t)h_j + \mathcal{O}(\lVert \textbf{h}\rVert^2)
\end{equation}
that is 
\begin{equation}
\textbf{u}(\textbf{y},t) = \textbf{u}(\textbf{x},t) + \nabla \textbf{u}(\textbf{x},t)\cdot \textbf{h} + \mathcal{O}(\lVert \textbf{h}\rVert^2)
\label{eq: u expand }
\end{equation}
where $\nabla \textbf{u}(\textbf{x},t)\cdot \textbf{h}$ is a matrix multiplication with 
\begin{equation}
\textbf{h} = \begin{pmatrix}h_1\\h_2\\h_3\end{pmatrix}
\end{equation}
Let 
\begin{equation}
\textbf{D} = \frac{1}{2}\left(\nabla \textbf{u}+(\nabla\textbf{u})^T\right)
\quad\text{and}\quad
\textbf{S} = \frac{1}{2}\left(\nabla \textbf{u}-(\nabla\textbf{u})^T\right)
\end{equation}
then $\nabla \textbf{u} = \textbf{S} + \textbf{D}$, and
\begin{equation}
\begin{aligned}
\textbf{D}^T &= \frac{1}{2}\left(\nabla \textbf{u}+(\nabla\textbf{u})^T\right)^T
= \frac{1}{2}\left((\nabla \textbf{u})^T+\nabla\textbf{u}\right) &&= \textbf{D}
\\[6pt]
\textbf{S}^T &= \frac{1}{2}\left(\nabla \textbf{u}-(\nabla\textbf{u})^T\right)
=\frac{1}{2}\left((\nabla \textbf{u})^T-\nabla\textbf{u}\right) &&=  -\textbf{S}
\end{aligned}
\end{equation}
So that, here $\textbf{D}$ is a symmetric matrix $\textbf{D}^{T}=\textbf{D}$ and $S$ is a anti-symmetric matrix $\textbf{S}=-\textbf{S}^{T}$. 

By direct computation 
\begin{equation}
\textbf{S} = \frac{1}{2}\left(\nabla \textbf{u}-(\nabla\textbf{u})^T\right)
= \frac{1}{2}\begin{pmatrix}
0 & \mathbf{\xi}_3 & \mathbf{\xi}_2 \\
\mathbf{\xi}_3 & 0 & -\mathbf{\xi}_1 \\
-\mathbf{\xi}_2 & \mathbf{\xi}_1 & 0
\end{pmatrix},\quad\text{where }
\mathbf{\xi} = \begin{pmatrix}\mathbf{\xi}_1\\\mathbf{\xi}_2\\\mathbf{\xi}_3\end{pmatrix}
= \nabla \times \textbf{u}
\end{equation}
Then $\displaystyle \textbf{S}\cdot \textbf{h} = \frac{1}{2}\mathbf{\xi} \cdot \textbf{h}$, i.e. 
\begin{equation}
...
\end{equation}
then substituting into $(\ref{eq: u expand })$ we have
\begin{equation}
\textbf{u}(\textbf{y},t) = \textbf{u}(\textbf{x},t) + \textbf{D}(\textbf{x},t)\cdot \textbf{h} + \frac{1}{2}\mathbf{\xi}(\textbf{x},t)\cdot \textbf{h} + \mathcal{O}\left(\lVert \textbf{h}\rVert^2\right),
\end{equation}


\begin{quote}
	Rmk 1:
Let $\displaystyle \Psi((\textbf{x},t),\textbf{h})=\frac{1}{2}\big(\textbf{D}(\textbf{x},t)\textbf{h}\big)\cdot\textbf{h}$,or

\begin{equation}
\Psi((\textbf{x},t),\textbf{h}) = \frac{1}{2}\textbf{h}^{T}\textbf{D}(\textbf{x},t)\textbf{h}
= \sum_{i,j=1}^{3}\frac{1}{2}h_{i}d_{i,j}h_{j}
\end{equation}
be the quadratic form associate with $\textbf{D}$, where $(\textbf{D})_{i,j} = d_{i,j}$, then
\begin{equation}
\begin{aligned}
\frac{\partial \Psi}{\partial h_{k}}
&= \frac{1}{2}\sum_{i,j=1}^{3}\frac{\partial}{\partial h_{k}}\left(h_{i}d_{i,j}h_{j}\right)\\
&= \frac{1}{2}\sum_{i,j=1}^{3}\left(\delta_{i,k}d_{i,j}h_{j} + h_{i}d_{i,j}\delta_{j,k}\right)\\
&= \frac{1}{2}\sum_{i,j=1}^{3}\delta_{i,k}d_{i,j}h_{j}
+ \frac{1}{2}\sum_{i,j=1}^{3} h_{i}d_{i,j}\delta_{j,k}\\
&= \frac{1}{2}\sum_{j=1}^{3}d_{k,j}h_{j}
+ \frac{1}{2}\sum_{i=1}^{3} h_{i}d_{i,k}\\
&= \frac{1}{2}\sum_{j=1}^{3}d_{k,j}h_{j}
+ \frac{1}{2}\sum_{j=1}^{3} h_{j}d_{j,k}\\
&= \frac{1}{2}\sum_{j=1}^{3}(d_{k,j} +  d_{j,k})h_{j}\\
\end{aligned}
\end{equation}
since $\textbf{D}$ is symmetric ($d_{k,j}=d_{j,k}$), we have
\begin{equation}
\frac{\partial \Psi}{\partial h_{k}}
= \frac{1}{2}\sum_{j=1}^{3}(d_{k,j} + d_{j,k})h_{j}
= \frac{1}{2}\sum_{j=1}^{3}2(d_{k,j} + d_{k,j})h_{j}
= \sum_{j=1}^{3}d_{k,j}h_{j}
\end{equation}
in vector representation, we have
\begin{equation}
\nabla_{\textbf{h}} \Psi((\textbf{x},t), \textbf{h}) = \textbf{D}(\textbf{x},t)\cdot \textbf{h}.
\end{equation}
We call $\textbf{D}$ the \textit{deformation tensor}.
\end{quote}

\begin{quote}
	Rmk 2:
Since $\textbf{D}$ is symmetric, $\textbf{D}$ is diagonoalizable, that is $\exists$ orthorgonal matrix $\textbf{U}$, such that
\begin{equation}
\widetilde{\textbf{U}} = \textbf{U}\textbf{D}\textbf{U}^{T}
= \begin{pmatrix}
d_1 & 0 & 0\\
0 & d_2 & 0\\
0 & 0 & d_3
\end{pmatrix}
\end{equation}
and $\textbf{U}^{T}\textbf{U} = \textbf{I} = \textbf{U}\textbf{U}^{T}$
\end{quote}

