then plugin to the integral
$$
\begin{aligned}
\frac{d}{dt}\int_{W_t} \rho f dV 
&= \int_W \left(
	\frac{D(\rho f)}{D t} + (\rho f) \operatorname{div}_y (\textbf{u})
	\right)\,dV\\
&= \int_W \left(
	\rho \frac{Df}{Dt} -  (\rho f) \operatorname{div}( \textbf{u}) + (\rho f) \operatorname{div}_y (\textbf{u})
	\right)\,dV\\
&= \int_W \left( \rho \frac{Df}{Dt}	\right)\,dV\\
\end{aligned}
$$

we get
$$
\frac{d}{dt}\int_{W_t} \rho f dV 
= \int_W \left( \rho \frac{Df}{Dt}	\right)\,dV,\quad\text{$\forall f$ is smooth function}
$$

> Notice that:
> $$
> \frac{d}{dt}\int_{W_t} \rho f dV 
> = \int_W \left( \rho \frac{Df}{Dt}	\right)\,dV
> $$
> so when we consider a vector fucntion $\textbf{u}$, we can write 
> $$
> \begin{aligned}
> \frac{d}{dt}\int_{W_t} \rho \textbf{u} dV 
> &= \frac{d}{dt}\int_{W_t} \rho (u_1,u_2,u_3) dV\\  
> &= \left(\frac{d}{dt}\int_{W_t} \rho u_1 dV, \frac{d}{dt}\int_{W_t} \rho u_2 dV,\frac{d}{dt}\int_{W_t} \rho u_3 dV\right)\\
> &= \left(
> 	\int_W \left( \rho \frac{Du_1}{Dt}	\right)\,dV,
> 	\int_W \left( \rho \frac{Du_2}{Dt}	\right)\,dV,
> 	\int_W \left( \rho \frac{Du_3}{Dt}	\right)\,dV
> 	\right)\\
> &= \int_W \left(
> 	\rho \frac{Du_1}{Dt},
> 	\rho \frac{Du_2}{Dt}
> 	\rho \frac{Du_3}{Dt}
> 	\right)\,dV\\
> &= \int_W \rho \frac{D}{Dt}\left(u_1,u_2,u_3\right)\,dV\\
> &= \int_W \rho \frac{D\textbf{u}}{Dt}\,dV\\
> \end{aligned}
> $$
> 
> 

Now we rewrite BM3
$$
\frac{d}{dt} \int_{W_t} \rho \textbf{u} dV = -\int_{W_t} \nabla pdV + \int_{W_t} \rho \textbf{b}dV
$$
to be
$$
\frac{d}{dt} \int_{W_t} \rho \textbf{u} dV + \int_{W_t} \nabla pdV - \int_{W_t} \rho \textbf{b}dV = 0
$$
then using the result from above
$$
\begin{aligned}
0 &= \frac{d}{dt} \int_{W_t} \rho \textbf{u} dV + \int_{W_t} \nabla pdV - \int_{W_t} \rho \textbf{b}dV\\
0 &=\int_{W_t} \rho \frac{D\textbf{u}}{Dt} dV + \int_{W_t} \nabla pdV - \int_{W_t} \rho \textbf{b}dV\\
0 &= \int_{W_t} \left(\rho \frac{D\textbf{u}}{Dt} dV + \nabla pdV - \rho \textbf{b}\right)dV,\quad \forall W_t
\end{aligned}
$$
imply 
$$
\rho \frac{D\textbf{u}}{Dt} dV + \nabla pdV - \rho \textbf{b} = 0
$$
which is just BM1, this means BM3 is equivalent to BM1. 

Similarly, 
$$
\frac{d}{dt}\int_{W} \rho \textbf{u} dV= \int_{\partial W_t} p\textbf{n} + \rho (\textbf{u}\cdot \textbf{n})\textbf{u} dA + \int_{W}\rho \textbf{b} dV
$$
 so that 
$$
\text{BM1} \Leftrightarrow \text{BM2} \Leftrightarrow \text{BM3}
$$
By an arrgument similart ot the proof of the transport theorem, for any smooth function $f:D\times [0,T] \to \mathbb{R}$, we have
$$
\frac{d}{dt}\left(\int_{W_t} fdV\right) 
= \int_{W_t} \left(\frac{Df}{Dt} + f(\operatorname{div}\textbf{u})\right) dV
\label{eq:transport thm without mass density 1}
$$

or in the other form as the textbook
$$
\frac{d}{dt}\int_{W_t} f dV = \int_{W_t} \left(\frac{\partial f}{\partial t} + \operatorname{div}(f\textbf{u})\right)dV,
\label{eq:transport thm without mass density 2}
$$
since $\displaystyle\frac{Df}{Dt} = \frac{\partial f}{\partial t} + \textbf{u}\cdot \nabla f$, and these 2 equations $(\ref{eq:transport thm without mass density 1})$ and $(\ref{eq:transport thm without mass density 2})$ is called the *Transport theorem without mass density*.

> Rmk: 
>
> Here we consider the *Transport theorem* (with mass density):
> $$
> \frac{d}{dt}\int_{W_t} \rho f dV = \int_{W_t} \rho \frac{Df}{Dt} dV,
> $$
> if we take $\rho$ to be a constant (ex: $\rho =1$), we have
> $$
> \frac{d}{dt}\int_{W_t} f dV = \int_{W_t} \frac{Df}{Dt} dV,
> $$
> however compare to the equation without no mass density  $(\ref{eq:transport thm without mass density 1})$â€‹, 
> $$
> \frac{d}{dt}\left(\int_{W_t} fdV\right) 
> = \int_{W_t} \frac{Df}{Dt}dV + \int_{W_t}f(\operatorname{div}\textbf{u}) dV
> $$
> we have an extra term contain $f(\operatorname{div}\textbf{u})$. **BUT**, if  we consider more carefully, the mass density $\rho$ here must satisfy the continuity equation, i.e.
> $$
> \rho_t + \operatorname{div}(\rho \textbf{u}) = 0
> $$
> so that if mass density is a constant (ex: $\rho = 1 $), we have
> $$
> \begin{aligned}
> \rho_t + \operatorname{div}(\rho \textbf{u}) = 0 + \operatorname{div}(\textbf{u}) = 0
> \end{aligned}
> $$
> so that $\operatorname{div}\textbf{u} = 0$, which means the extra term vanishing, and the *transport theorem with mass density* and *transport theorem without mass density* are equivalent.