
% Sets the document class and font size
\documentclass[12pt]{article}
\usepackage[a4paper, margin=1in, top=0.8in, bottom=0.9in]{geometry}

\usepackage[utf8]{inputenc}    % Input encoding
\usepackage[T1]{fontenc}       % Font encoding
\usepackage{fontspec}          % font encoding

% Advanced math typesetting
\usepackage{amsmath}
\usepackage{amssymb}
\usepackage{mathtools}
\usepackage{physics}

% Symbols and Text
\usepackage{bbold}     % bold font
\usepackage{ulem}      % strikethrough
\usepackage{listings}  % Source code listing
\usepackage{import}    % Importing code and other documents

% graphics
\usepackage[dvipsnames]{xcolor}
\usepackage{graphicx}
\usepackage{tikz}
\usepackage{pgfplots}
\usepackage{tcolorbox}
%\usepackage{changepage}

% figure
\usepackage{float}
\usepackage{subfigure}

\usepackage{hyperref}  % Hyperlinks in the document
\hypersetup{
    colorlinks=true,
    linkcolor=Blue,
    filecolor=red,
    urlcolor=Blue,
    citecolor=blue,
    pdftitle={Article},
    pdfauthor={Author},
}

\usepackage{xeCJK}               % Chinese, Japanese, and Korean characters
\setCJKfamilyfont{kai}{標楷體}    % Chinese font

\usepackage{subfiles}  % Best loaded last in the preamble
\usepackage{titlesec}  % fortitle

\titleclass{\subsubsubsection}{straight}[\subsection]

\newcounter{subsubsubsection}[subsubsection]
\renewcommand\thesubsubsubsection{\thesubsubsection.\arabic{subsubsubsection}}
\renewcommand\theparagraph{\thesubsubsubsection.\arabic{paragraph}} % optional; useful if paragraphs are to be numbered

\titleformat{\subsubsubsection}
  {\normalfont\normalsize\bfseries}{\thesubsubsubsection}{1em}{}
\titlespacing*{\subsubsubsection}
{0pt}{3.25ex plus 1ex minus .2ex}{1.5ex plus .2ex}

\makeatletter
\renewcommand\paragraph{
    \@startsection{paragraph}{5}{\z@}{3.25ex\@plus1ex\@minus.2ex}{-1em}{\normalfont\normalsize\bfseries}
}
\renewcommand\subparagraph{
    \@startsection{subparagraph}{6}{\parindent}{3.25ex\@plus1ex\@minus.2ex}{-1em}{\normalfont\normalsize\bfseries}
}
\def\toclevel@subsubsubsection{4}
\def\toclevel@paragraph{5}
\def\toclevel@paragraph{6}
\def\l@subsubsubsection{\@dottedtocline{4}{7em}{4em}}
\def\l@paragraph{\@dottedtocline{5}{10em}{5em}}
\def\l@subparagraph{\@dottedtocline{6}{14em}{6em}}
\makeatother

\setcounter{secnumdepth}{4}
\setcounter{tocdepth}{4}

\usepackage{fancyhdr}
\pagestyle{fancy}

\title{Note: Levi-Civita symbol}
\date{\today}
\author{Chang-Mao Yang 楊長茂}

\begin{document}
%================================================================================================
\maketitle
\tableofcontents
\section{Definition}
In three dimensions, the Levi-Civita symbol is defined by:
\begin{equation}
\varepsilon _{ijk} =
\begin{cases}
+1	&	\text{if $(i,j,k)$ is $(1,2,3)$, $(2,3,1)$ or $(3,1,2)$}\\
-1	&	\text{if $(i,j,k)$ is $(3,2,1)$, $(2,1,3)$ or $(2,1,3)$}\\
\;\;\,0&\text{if $i=j$, $i=k$ or $k=i$}
\end{cases}
\end{equation}
That is, $\varepsilon_{ijk}$ is $1$ if $(i,j,k)$ is an even permutation of $(1,2,3)$, $−1$ if it is an odd permutation, and $0$​ if any index is repeated.

\section{Properties}

\subsection{Product}


\begin{equation}
\begin{aligned}
\varepsilon _{ijk}\varepsilon _{lmn}
&=\begin{vmatrix}
\delta _{il}&\delta _{im}&\delta _{in}\\
\delta _{jl}&\delta _{jm}&\delta _{jn}\\
\delta _{kl}&\delta _{km}&\delta _{kn}
\end{vmatrix}\\[6pt]
&=\delta _{il} \left(\delta _{jm}\delta _{kn}-\delta _{jn}\delta _{km}\right)
-\delta _{im} \left(\delta _{jl}\delta _{kn}-\delta _{jn}\delta _{kl}\right)
+\delta _{in} \left(\delta _{jl}\delta _{km}-\delta _{jm}\delta _{kl}\right).
\end{aligned}
\end{equation}

\subsection{Special cases} % H3 title


\begin{equation}
\sum _{i=1}^{3}\varepsilon _{ijk}\varepsilon _{imn}=\delta _{jm}\delta _{kn}-\delta _{jn}\delta _{km}
\end{equation}

\subsubsection{Proof of special cases (method 1)}

Using the properties of product
\begin{equation}
\begin{aligned}
\sum _{i=1}^{3}\varepsilon _{ijk}\varepsilon _{imn}
&= \sum _{i=1}^{3}\begin{vmatrix}
\delta _{ii}&\delta _{im}&\delta _{in}\\
\delta _{ji}&\delta _{jm}&\delta _{jn}\\
\delta _{ki}&\delta _{km}&\delta _{kn}
\end{vmatrix}\\[6pt]
&= \sum _{i=1}^{3}\bigg(\delta _{ii} \left(\delta _{jm}\delta _{kn}-\delta _{jn}\delta _{km}\right)
-\delta _{im} \left(\delta _{ji}\delta _{kn}-\delta _{jn}\delta _{ki}\right)
+\delta _{in} \left(\delta _{ji}\delta _{km}-\delta _{jm}\delta _{ki}\right)\bigg)\\
&= \left(\delta _{jm}\delta _{kn}-\delta _{jn}\delta _{km}\right)  \sum _{i=1}^{3}\delta _{ii}
+ \sum _{i=1}^{3}\bigg(-\delta _{im} \left(\delta _{ji}\delta _{kn}-\delta _{jn}\delta _{ki}\right)
+\delta _{in} \left(\delta _{ji}\delta _{km}-\delta _{jm}\delta _{ki}\right)\bigg)\\
&= 3\cdot\left(\delta _{jm}\delta _{kn}-\delta _{jn}\delta _{km}\right)
+ \sum _{i=1}^{3}\left(
-\delta _{im}\delta _{ji}\delta _{kn} + \delta _{im}\delta _{jn}\delta _{ki}
+\delta _{in}\delta _{ji}\delta _{km} - \delta _{in}\delta _{jm}\delta _{ki}
\right)\\[6pt]
&= 3\cdot\left(\delta _{jm}\delta _{kn}-\delta _{jn}\delta _{km}\right)
-\delta _{jm}\delta _{kn} + \delta _{km}\delta _{jn}
+\delta _{jn}\delta _{km} - \delta _{kn}\delta _{jm}\\[6pt]
&= 3\cdot\left(\delta _{jm}\delta _{kn}-\delta _{jn}\delta _{km}\right)
-2\delta _{jm}\delta _{kn} + 2\delta _{km}\delta _{jn}\\[6pt]
&= \delta _{jm}\delta _{kn}-\delta _{km}\delta _{jn}
\end{aligned}
\end{equation}


\subsubsection{Proof of special cases (method 2)}
Claim $\varepsilon_{i,j,k}\varepsilon_{i,m,n} = \delta_{jm}\delta_{kn} - \delta_{jn}\delta_{km}$, where $i,j,k,m,n\in\{1,2,3\}$. WLOG, we may assume $\{i,j,k\}$ are all distinct and $\{i,m,n\}$ are all distinct.
\begin{enumerate}

\item If $j=m$ then $k=n$ and $j\neq k$, and we can rewrite
\begin{equation}
\varepsilon_{i,j,k}\varepsilon_{i,m,n} = \varepsilon_{i,j,k}\varepsilon_{i,j,k} = 1 = \delta_{jm}\delta_{kn} - \delta_{jn}\delta_{km}.
\end{equation}

\item If $j=n$ then $k=m$ and $j\neq k$, and we can rewrite 
\begin{equation}
\varepsilon_{i,j,k}\varepsilon_{i,m,n} = \varepsilon_{i,j,k}\varepsilon_{i,k,j} = -\varepsilon_{i,j,k}\varepsilon_{i,j,k} = -1 = \delta_{jm}\delta_{kn} - \delta_{jn}\delta_{km}.
\end{equation}
\end{enumerate}


\newpage
\subsubsection{Proof of special cases (method 3)} 
Consider $\varepsilon_{i,j,k}\varepsilon_{i,m,n}$ for $i=1,2,3$, we have 

\begin{enumerate}

\item When $i=1$, the indices $(j,k)$ and $(m,n)$ can only be $(2,3)$ or $(3,2)$, otherwise this term will be zero.
\begin{equation}
\varepsilon_{1,j,k}\varepsilon_{1,m,n} : \begin{cases}
\varepsilon_{1,2,3}\varepsilon_{1,2,3}&=1,\\
\varepsilon_{1,2,3}\varepsilon_{1,3,2}&=-1,\\
\varepsilon_{1,3,2}\varepsilon_{1,2,3}&=-1,\\
\varepsilon_{1,3,2}\varepsilon_{1,3,2}&=1.
\end{cases}
\end{equation}
Above result shows that: $\varepsilon_{1,j,k}\varepsilon_{1,m,n}=1$ if $j=m$ and $k=n$; $\varepsilon_{1,j,k}\varepsilon_{1,m,n}=-1$ if $j=n$ and $k=m$. So we can write this term to be 
\begin{equation}
\varepsilon_{1,j,k}\varepsilon_{1,m,n} = \delta_{jm}\delta_{kn} - \delta_{jn}\delta_{km}.
\end{equation}
\hrule

\item When $i=2$, the indices $(j,k)$ and $(m,n)$ can only be $(1,3)$ or $(3,1)$, otherwise this term will be zero.
\begin{equation}
\varepsilon_{2,j,k}\varepsilon_{2,m,n} : \begin{cases}
\varepsilon_{2,1,3}\varepsilon_{2,1,3}&=1,\\
\varepsilon_{2,1,3}\varepsilon_{2,3,1}&=-1,\\
\varepsilon_{2,3,1}\varepsilon_{2,1,3}&=-1,\\
\varepsilon_{2,3,1}\varepsilon_{2,3,1}&=1.
\end{cases}
\end{equation}
Above result shows that: $\varepsilon_{2,j,k}\varepsilon_{2,m,n}=1$ if $j=m$ and $k=n$; $\varepsilon_{2,j,k}\varepsilon_{2,m,n}=-1$ if $j=n$ and $k=m$. So we can write this term to be 
\begin{equation}
\varepsilon_{2,j,k}\varepsilon_{2,m,n} = \delta_{jm}\delta_{kn} - \delta_{jn}\delta_{km}.
\end{equation}
\hrule

\item When $i=3$, the indices $(j,k)$ and $(m,n)$ can only be $(1,2)$ or $(2,1)$, otherwise this term will be zero.
\begin{equation}
\varepsilon_{3,j,k}\varepsilon_{3,m,n} : \begin{cases}
\varepsilon_{3,1,2}\varepsilon_{3,1,2}&=1,\\
\varepsilon_{3,1,2}\varepsilon_{3,2,1}&=-1,\\
\varepsilon_{3,2,1}\varepsilon_{3,1,2}&=-1,\\
\varepsilon_{3,2,1}\varepsilon_{3,2,1}&=1.
\end{cases}
\end{equation}
Above result shows that: $\varepsilon_{3,j,k}\varepsilon_{3,m,n}=1$ if $j=m$ and $k=n$; $\varepsilon_{3,j,k}\varepsilon_{3,m,n}=-1$ if $j=n$ and $k=m$. So we can write this term to be 
\begin{equation}
\varepsilon_{3,j,k}\varepsilon_{3,m,n} = \delta_{jm}\delta_{kn} - \delta_{jn}\delta_{km}.
\end{equation}
\hrule

\end{enumerate}
Then summing over $i$, we have  
\begin{equation}
\sum_{i=1}^{3}\varepsilon_{i,j,k}\varepsilon_{i,m,n} = 
\varepsilon_{1,j,k}\varepsilon_{1,m,n}
+ \varepsilon_{2,j,k}\varepsilon_{2,m,n}
+ \varepsilon_{3,j,k}\varepsilon_{3,m,n}.
\end{equation}
We can observe that, at most one of the three terms will be different from zero. Using the above conclusion, we can write 
\begin{equation}
\sum_{i=1}^{3}\varepsilon_{i,j,k}\varepsilon_{i,m,n} = \delta_{jm}\delta_{kn} - \delta_{jn}\delta_{km}.
\end{equation}

\newpage
If we write down all the possibility if $\varepsilon_{i,j,k}\varepsilon_{i,m,n}$ for $i,j,k,m,n\in\{1,2,3\}$, we have
\begin{equation}\hspace{-1cm}
\begin{aligned}
&&\varepsilon_{1,1,1}\varepsilon_{1,1,1}=0&&\varepsilon_{2,1,1}\varepsilon_{2,1,1}=0&&\varepsilon_{3,1,1}\varepsilon_{3,1,1}=0&&\varepsilon_{1,1,1}\varepsilon_{1,1,2}=0&&\varepsilon_{2,1,1}\varepsilon_{2,1,2}=0&&\varepsilon_{3,1,1}\varepsilon_{3,1,2}=0\\
&&\varepsilon_{1,1,1}\varepsilon_{1,1,3}=0&&\varepsilon_{2,1,1}\varepsilon_{2,1,3}=0&&\varepsilon_{3,1,1}\varepsilon_{3,1,3}=0&&\varepsilon_{1,1,1}\varepsilon_{1,2,1}=0&&\varepsilon_{2,1,1}\varepsilon_{2,2,1}=0&&\varepsilon_{3,1,1}\varepsilon_{3,2,1}=0\\
&&\varepsilon_{1,1,1}\varepsilon_{1,2,2}=0&&\varepsilon_{2,1,1}\varepsilon_{2,2,2}=0&&\varepsilon_{3,1,1}\varepsilon_{3,2,2}=0&&\varepsilon_{1,1,1}\varepsilon_{1,2,3}=0&&\varepsilon_{2,1,1}\varepsilon_{2,2,3}=0&&\varepsilon_{3,1,1}\varepsilon_{3,2,3}=0\\
&&\varepsilon_{1,1,1}\varepsilon_{1,3,1}=0&&\varepsilon_{2,1,1}\varepsilon_{2,3,1}=0&&\varepsilon_{3,1,1}\varepsilon_{3,3,1}=0&&\varepsilon_{1,1,1}\varepsilon_{1,3,2}=0&&\varepsilon_{2,1,1}\varepsilon_{2,3,2}=0&&\varepsilon_{3,1,1}\varepsilon_{3,3,2}=0\\
&&\varepsilon_{1,1,1}\varepsilon_{1,3,3}=0&&\varepsilon_{2,1,1}\varepsilon_{2,3,3}=0&&\varepsilon_{3,1,1}\varepsilon_{3,3,3}=0&&\varepsilon_{1,1,2}\varepsilon_{1,1,1}=0&&\varepsilon_{2,1,2}\varepsilon_{2,1,1}=0&&\varepsilon_{3,1,2}\varepsilon_{3,1,1}=0\\
&&\varepsilon_{1,1,2}\varepsilon_{1,1,2}=0&&\varepsilon_{2,1,2}\varepsilon_{2,1,2}=0&&{\color{red}\varepsilon_{3,1,2}\varepsilon_{3,1,2}=1}
&&\varepsilon_{1,1,2}\varepsilon_{1,1,3}=0&&\varepsilon_{2,1,2}\varepsilon_{2,1,3}=0&&\varepsilon_{3,1,2}\varepsilon_{3,1,3}=0\\
&&\varepsilon_{1,1,2}\varepsilon_{1,2,1}=0&&\varepsilon_{2,1,2}\varepsilon_{2,2,1}=0&&{\color{red}\varepsilon_{3,1,2}\varepsilon_{3,2,1}=-1}
&&\varepsilon_{1,1,2}\varepsilon_{1,2,2}=0&&\varepsilon_{2,1,2}\varepsilon_{2,2,2}=0&&\varepsilon_{3,1,2}\varepsilon_{3,2,2}=0\\
&&\varepsilon_{1,1,2}\varepsilon_{1,2,3}=0&&\varepsilon_{2,1,2}\varepsilon_{2,2,3}=0&&\varepsilon_{3,1,2}\varepsilon_{3,2,3}=0&&\varepsilon_{1,1,2}\varepsilon_{1,3,1}=0&&\varepsilon_{2,1,2}\varepsilon_{2,3,1}=0&&\varepsilon_{3,1,2}\varepsilon_{3,3,1}=0\\
&&\varepsilon_{1,1,2}\varepsilon_{1,3,2}=0&&\varepsilon_{2,1,2}\varepsilon_{2,3,2}=0&&\varepsilon_{3,1,2}\varepsilon_{3,3,2}=0&&\varepsilon_{1,1,2}\varepsilon_{1,3,3}=0&&\varepsilon_{2,1,2}\varepsilon_{2,3,3}=0&&\varepsilon_{3,1,2}\varepsilon_{3,3,3}=0\\
&&\varepsilon_{1,1,3}\varepsilon_{1,1,1}=0&&\varepsilon_{2,1,3}\varepsilon_{2,1,1}=0&&\varepsilon_{3,1,3}\varepsilon_{3,1,1}=0&&\varepsilon_{1,1,3}\varepsilon_{1,1,2}=0&&\varepsilon_{2,1,3}\varepsilon_{2,1,2}=0&&\varepsilon_{3,1,3}\varepsilon_{3,1,2}=0\\
&&\varepsilon_{1,1,3}\varepsilon_{1,1,3}=0&&{\color{red}\varepsilon_{2,1,3}\varepsilon_{2,1,3}=1}
&&\varepsilon_{3,1,3}\varepsilon_{3,1,3}=0&&\varepsilon_{1,1,3}\varepsilon_{1,2,1}=0&&\varepsilon_{2,1,3}\varepsilon_{2,2,1}=0&&\varepsilon_{3,1,3}\varepsilon_{3,2,1}=0\\
&&\varepsilon_{1,1,3}\varepsilon_{1,2,2}=0&&\varepsilon_{2,1,3}\varepsilon_{2,2,2}=0&&\varepsilon_{3,1,3}\varepsilon_{3,2,2}=0&&\varepsilon_{1,1,3}\varepsilon_{1,2,3}=0&&\varepsilon_{2,1,3}\varepsilon_{2,2,3}=0&&\varepsilon_{3,1,3}\varepsilon_{3,2,3}=0\\
&&\varepsilon_{1,1,3}\varepsilon_{1,3,1}=0&&{\color{red}\varepsilon_{2,1,3}\varepsilon_{2,3,1}=-1}
&&\varepsilon_{3,1,3}\varepsilon_{3,3,1}=0&&\varepsilon_{1,1,3}\varepsilon_{1,3,2}=0&&\varepsilon_{2,1,3}\varepsilon_{2,3,2}=0&&\varepsilon_{3,1,3}\varepsilon_{3,3,2}=0\\
&&\varepsilon_{1,1,3}\varepsilon_{1,3,3}=0&&\varepsilon_{2,1,3}\varepsilon_{2,3,3}=0&&\varepsilon_{3,1,3}\varepsilon_{3,3,3}=0&&\varepsilon_{1,2,1}\varepsilon_{1,1,1}=0&&\varepsilon_{2,2,1}\varepsilon_{2,1,1}=0&&\varepsilon_{3,2,1}\varepsilon_{3,1,1}=0\\
&&\varepsilon_{1,2,1}\varepsilon_{1,1,2}=0&&\varepsilon_{2,2,1}\varepsilon_{2,1,2}=0&&{\color{red}\varepsilon_{3,2,1}\varepsilon_{3,1,2}=-1}
&&\varepsilon_{1,2,1}\varepsilon_{1,1,3}=0&&\varepsilon_{2,2,1}\varepsilon_{2,1,3}=0&&\varepsilon_{3,2,1}\varepsilon_{3,1,3}=0\\
&&\varepsilon_{1,2,1}\varepsilon_{1,2,1}=0&&\varepsilon_{2,2,1}\varepsilon_{2,2,1}=0&&{\color{red}\varepsilon_{3,2,1}\varepsilon_{3,2,1}=1}
&&\varepsilon_{1,2,1}\varepsilon_{1,2,2}=0&&\varepsilon_{2,2,1}\varepsilon_{2,2,2}=0&&\varepsilon_{3,2,1}\varepsilon_{3,2,2}=0\\
&&\varepsilon_{1,2,1}\varepsilon_{1,2,3}=0&&\varepsilon_{2,2,1}\varepsilon_{2,2,3}=0&&\varepsilon_{3,2,1}\varepsilon_{3,2,3}=0&&\varepsilon_{1,2,1}\varepsilon_{1,3,1}=0&&\varepsilon_{2,2,1}\varepsilon_{2,3,1}=0&&\varepsilon_{3,2,1}\varepsilon_{3,3,1}=0\\
&&\varepsilon_{1,2,1}\varepsilon_{1,3,2}=0&&\varepsilon_{2,2,1}\varepsilon_{2,3,2}=0&&\varepsilon_{3,2,1}\varepsilon_{3,3,2}=0&&\varepsilon_{1,2,1}\varepsilon_{1,3,3}=0&&\varepsilon_{2,2,1}\varepsilon_{2,3,3}=0&&\varepsilon_{3,2,1}\varepsilon_{3,3,3}=0\\
&&\varepsilon_{1,2,2}\varepsilon_{1,1,1}=0&&\varepsilon_{2,2,2}\varepsilon_{2,1,1}=0&&\varepsilon_{3,2,2}\varepsilon_{3,1,1}=0&&\varepsilon_{1,2,2}\varepsilon_{1,1,2}=0&&\varepsilon_{2,2,2}\varepsilon_{2,1,2}=0&&\varepsilon_{3,2,2}\varepsilon_{3,1,2}=0\\
&&\varepsilon_{1,2,2}\varepsilon_{1,1,3}=0&&\varepsilon_{2,2,2}\varepsilon_{2,1,3}=0&&\varepsilon_{3,2,2}\varepsilon_{3,1,3}=0&&\varepsilon_{1,2,2}\varepsilon_{1,2,1}=0&&\varepsilon_{2,2,2}\varepsilon_{2,2,1}=0&&\varepsilon_{3,2,2}\varepsilon_{3,2,1}=0\\
&&\varepsilon_{1,2,2}\varepsilon_{1,2,2}=0&&\varepsilon_{2,2,2}\varepsilon_{2,2,2}=0&&\varepsilon_{3,2,2}\varepsilon_{3,2,2}=0&&\varepsilon_{1,2,2}\varepsilon_{1,2,3}=0&&\varepsilon_{2,2,2}\varepsilon_{2,2,3}=0&&\varepsilon_{3,2,2}\varepsilon_{3,2,3}=0\\
&&\varepsilon_{1,2,2}\varepsilon_{1,3,1}=0&&\varepsilon_{2,2,2}\varepsilon_{2,3,1}=0&&\varepsilon_{3,2,2}\varepsilon_{3,3,1}=0&&\varepsilon_{1,2,2}\varepsilon_{1,3,2}=0&&\varepsilon_{2,2,2}\varepsilon_{2,3,2}=0&&\varepsilon_{3,2,2}\varepsilon_{3,3,2}=0\\
&&\varepsilon_{1,2,2}\varepsilon_{1,3,3}=0&&\varepsilon_{2,2,2}\varepsilon_{2,3,3}=0&&\varepsilon_{3,2,2}\varepsilon_{3,3,3}=0&&\varepsilon_{1,2,3}\varepsilon_{1,1,1}=0&&\varepsilon_{2,2,3}\varepsilon_{2,1,1}=0&&\varepsilon_{3,2,3}\varepsilon_{3,1,1}=0\\
&&\varepsilon_{1,2,3}\varepsilon_{1,1,2}=0&&\varepsilon_{2,2,3}\varepsilon_{2,1,2}=0&&\varepsilon_{3,2,3}\varepsilon_{3,1,2}=0&&\varepsilon_{1,2,3}\varepsilon_{1,1,3}=0&&\varepsilon_{2,2,3}\varepsilon_{2,1,3}=0&&\varepsilon_{3,2,3}\varepsilon_{3,1,3}=0\\
&&\varepsilon_{1,2,3}\varepsilon_{1,2,1}=0&&\varepsilon_{2,2,3}\varepsilon_{2,2,1}=0&&\varepsilon_{3,2,3}\varepsilon_{3,2,1}=0&&\varepsilon_{1,2,3}\varepsilon_{1,2,2}=0&&\varepsilon_{2,2,3}\varepsilon_{2,2,2}=0&&\varepsilon_{3,2,3}\varepsilon_{3,2,2}=0\\
&&{\color{red}\varepsilon_{1,2,3}\varepsilon_{1,2,3}=1}
&&\varepsilon_{2,2,3}\varepsilon_{2,2,3}=0&&\varepsilon_{3,2,3}\varepsilon_{3,2,3}=0&&\varepsilon_{1,2,3}\varepsilon_{1,3,1}=0&&\varepsilon_{2,2,3}\varepsilon_{2,3,1}=0&&\varepsilon_{3,2,3}\varepsilon_{3,3,1}=0\\
&&{\color{red}\varepsilon_{1,2,3}\varepsilon_{1,3,2}=-1}
&&\varepsilon_{2,2,3}\varepsilon_{2,3,2}=0&&\varepsilon_{3,2,3}\varepsilon_{3,3,2}=0&&\varepsilon_{1,2,3}\varepsilon_{1,3,3}=0&&\varepsilon_{2,2,3}\varepsilon_{2,3,3}=0&&\varepsilon_{3,2,3}\varepsilon_{3,3,3}=0\\
&&\varepsilon_{1,3,1}\varepsilon_{1,1,1}=0&&\varepsilon_{2,3,1}\varepsilon_{2,1,1}=0&&\varepsilon_{3,3,1}\varepsilon_{3,1,1}=0&&\varepsilon_{1,3,1}\varepsilon_{1,1,2}=0&&\varepsilon_{2,3,1}\varepsilon_{2,1,2}=0&&\varepsilon_{3,3,1}\varepsilon_{3,1,2}=0\\
&&\varepsilon_{1,3,1}\varepsilon_{1,1,3}=0&&{\color{red}\varepsilon_{2,3,1}\varepsilon_{2,1,3}=-1}
&&\varepsilon_{3,3,1}\varepsilon_{3,1,3}=0&&\varepsilon_{1,3,1}\varepsilon_{1,2,1}=0&&\varepsilon_{2,3,1}\varepsilon_{2,2,1}=0&&\varepsilon_{3,3,1}\varepsilon_{3,2,1}=0\\
&&\varepsilon_{1,3,1}\varepsilon_{1,2,2}=0&&\varepsilon_{2,3,1}\varepsilon_{2,2,2}=0&&\varepsilon_{3,3,1}\varepsilon_{3,2,2}=0&&\varepsilon_{1,3,1}\varepsilon_{1,2,3}=0&&\varepsilon_{2,3,1}\varepsilon_{2,2,3}=0&&\varepsilon_{3,3,1}\varepsilon_{3,2,3}=0\\
&&\varepsilon_{1,3,1}\varepsilon_{1,3,1}=0&&{\color{red}\varepsilon_{2,3,1}\varepsilon_{2,3,1}=1}
&&\varepsilon_{3,3,1}\varepsilon_{3,3,1}=0&&\varepsilon_{1,3,1}\varepsilon_{1,3,2}=0&&\varepsilon_{2,3,1}\varepsilon_{2,3,2}=0&&\varepsilon_{3,3,1}\varepsilon_{3,3,2}=0\\
&&\varepsilon_{1,3,1}\varepsilon_{1,3,3}=0&&\varepsilon_{2,3,1}\varepsilon_{2,3,3}=0&&\varepsilon_{3,3,1}\varepsilon_{3,3,3}=0&&\varepsilon_{1,3,2}\varepsilon_{1,1,1}=0&&\varepsilon_{2,3,2}\varepsilon_{2,1,1}=0&&\varepsilon_{3,3,2}\varepsilon_{3,1,1}=0\\
&&\varepsilon_{1,3,2}\varepsilon_{1,1,2}=0&&\varepsilon_{2,3,2}\varepsilon_{2,1,2}=0&&\varepsilon_{3,3,2}\varepsilon_{3,1,2}=0&&\varepsilon_{1,3,2}\varepsilon_{1,1,3}=0&&\varepsilon_{2,3,2}\varepsilon_{2,1,3}=0&&\varepsilon_{3,3,2}\varepsilon_{3,1,3}=0\\
&&\varepsilon_{1,3,2}\varepsilon_{1,2,1}=0&&\varepsilon_{2,3,2}\varepsilon_{2,2,1}=0&&\varepsilon_{3,3,2}\varepsilon_{3,2,1}=0&&\varepsilon_{1,3,2}\varepsilon_{1,2,2}=0&&\varepsilon_{2,3,2}\varepsilon_{2,2,2}=0&&\varepsilon_{3,3,2}\varepsilon_{3,2,2}=0\\
&&{\color{red}\varepsilon_{1,3,2}\varepsilon_{1,2,3}=-1}
&&\varepsilon_{2,3,2}\varepsilon_{2,2,3}=0&&\varepsilon_{3,3,2}\varepsilon_{3,2,3}=0&&\varepsilon_{1,3,2}\varepsilon_{1,3,1}=0&&\varepsilon_{2,3,2}\varepsilon_{2,3,1}=0&&\varepsilon_{3,3,2}\varepsilon_{3,3,1}=0\\
&&{\color{red}\varepsilon_{1,3,2}\varepsilon_{1,3,2}=1}
&&\varepsilon_{2,3,2}\varepsilon_{2,3,2}=0&&\varepsilon_{3,3,2}\varepsilon_{3,3,2}=0&&\varepsilon_{1,3,2}\varepsilon_{1,3,3}=0&&\varepsilon_{2,3,2}\varepsilon_{2,3,3}=0&&\varepsilon_{3,3,2}\varepsilon_{3,3,3}=0\\
&&\varepsilon_{1,3,3}\varepsilon_{1,1,1}=0&&\varepsilon_{2,3,3}\varepsilon_{2,1,1}=0&&\varepsilon_{3,3,3}\varepsilon_{3,1,1}=0&&\varepsilon_{1,3,3}\varepsilon_{1,1,2}=0&&\varepsilon_{2,3,3}\varepsilon_{2,1,2}=0&&\varepsilon_{3,3,3}\varepsilon_{3,1,2}=0\\
&&\varepsilon_{1,3,3}\varepsilon_{1,1,3}=0&&\varepsilon_{2,3,3}\varepsilon_{2,1,3}=0&&\varepsilon_{3,3,3}\varepsilon_{3,1,3}=0&&\varepsilon_{1,3,3}\varepsilon_{1,2,1}=0&&\varepsilon_{2,3,3}\varepsilon_{2,2,1}=0&&\varepsilon_{3,3,3}\varepsilon_{3,2,1}=0\\
&&\varepsilon_{1,3,3}\varepsilon_{1,2,2}=0&&\varepsilon_{2,3,3}\varepsilon_{2,2,2}=0&&\varepsilon_{3,3,3}\varepsilon_{3,2,2}=0&&\varepsilon_{1,3,3}\varepsilon_{1,2,3}=0&&\varepsilon_{2,3,3}\varepsilon_{2,2,3}=0&&\varepsilon_{3,3,3}\varepsilon_{3,2,3}=0\\
&&\varepsilon_{1,3,3}\varepsilon_{1,3,1}=0&&\varepsilon_{2,3,3}\varepsilon_{2,3,1}=0&&\varepsilon_{3,3,3}\varepsilon_{3,3,1}=0&&\varepsilon_{1,3,3}\varepsilon_{1,3,2}=0&&\varepsilon_{2,3,3}\varepsilon_{2,3,2}=0&&\varepsilon_{3,3,3}\varepsilon_{3,3,2}=0\\
&&\varepsilon_{1,3,3}\varepsilon_{1,3,3}=0&&\varepsilon_{2,3,3}\varepsilon_{2,3,3}=0&&\varepsilon_{3,3,3}\varepsilon_{3,3,3}=0
\end{aligned}
\end{equation}
\newpage

\section{Application}
\subsection{Cross Product}
For $\hat{e}_1=(1,0,0)$, $\hat{e}_2=(0,1,0)$ and $\hat{e}_3=(0,0,1)$, we have
\begin{equation}
\hat{e}_j\times\hat{e}_k=\sum_{i=1}^3\varepsilon_{ijk}\hat{e}_i
\end{equation}

\noindent\fbox{\begin{minipage}{0.99\textwidth}
\noindent\textbf{proof}:
\begin{equation}
\begin{aligned}
\hat{e}_{1}\times\hat{e}_{1} &= \sum_{i=1}^{3}\varepsilon_{i,1,1}\hat{e}_i
= \varepsilon_{1,1,1}\hat{e}_{1}+\varepsilon_{2,1,1}\hat{e}_{2}+\varepsilon_{3,1,1}\hat{e}_{3}
= 0\\
\hat{e}_{1}\times\hat{e}_{2} &= \sum_{i=1}^{3}\varepsilon_{i,1,2}\hat{e}_i
= \varepsilon_{1,1,2}\hat{e}_{1}+\varepsilon_{2,1,2}\hat{e}_{2}+\varepsilon_{3,1,2}\hat{e}_{3}
= \hat{e}_{3}\\
\hat{e}_{1}\times\hat{e}_{3} &= \sum_{i=1}^{3}\varepsilon_{i,1,3}\hat{e}_i
= \varepsilon_{1,1,3}\hat{e}_{1}+\varepsilon_{2,1,3}\hat{e}_{2}+\varepsilon_{3,1,3}\hat{e}_{3}
= -\hat{e}_{2}\\
\hat{e}_{2}\times\hat{e}_{1} &= \sum_{i=1}^{3}\varepsilon_{i,2,1}\hat{e}_i
= \varepsilon_{1,2,1}\hat{e}_{1}+\varepsilon_{2,2,1}\hat{e}_{2}+\varepsilon_{3,2,1}\hat{e}_{3}
= -\hat{e}_{3}\\
\hat{e}_{2}\times\hat{e}_{2} &= \sum_{i=1}^{3}\varepsilon_{i,2,2}\hat{e}_i
= \varepsilon_{1,2,2}\hat{e}_{1}+\varepsilon_{2,2,2}\hat{e}_{2}+\varepsilon_{3,2,2}\hat{e}_{3}
= 0\\
\hat{e}_{2}\times\hat{e}_{3} &= \sum_{i=1}^{3}\varepsilon_{i,2,3}\hat{e}_i
= \varepsilon_{1,2,3}\hat{e}_{1}+\varepsilon_{2,2,3}\hat{e}_{2}+\varepsilon_{3,2,3}\hat{e}_{3}
= \hat{e}_{1}\\
\hat{e}_{3}\times\hat{e}_{1} &= \sum_{i=1}^{3}\varepsilon_{i,3,1}\hat{e}_i
= \varepsilon_{1,3,1}\hat{e}_{1}+\varepsilon_{2,3,1}\hat{e}_{2}+\varepsilon_{3,3,1}\hat{e}_{3}
= \hat{e}_{2}\\
\hat{e}_{3}\times\hat{e}_{2} &= \sum_{i=1}^{3}\varepsilon_{i,3,2}\hat{e}_i
= \varepsilon_{1,3,2}\hat{e}_{1}+\varepsilon_{2,3,2}\hat{e}_{2}+\varepsilon_{3,3,2}\hat{e}_{3}
= -\hat{e}_{1}\\
\hat{e}_{3}\times\hat{e}_{3} &= \sum_{i=1}^{3}\varepsilon_{i,3,3}\hat{e}_i
= \varepsilon_{1,3,3}\hat{e}_{1}+\varepsilon_{2,3,3}\hat{e}_{2}+\varepsilon_{3,3,3}\hat{e}_{3}
= 0\\
\end{aligned}
\end{equation}
\end{minipage}}
Then, for vectors $\vec{a}$ and $\vec{b}$, if we write $\displaystyle \vec{a} = \sum_{i=1}^{3}a_{i}\hat{e}_i$ and $\displaystyle \vec{b} = \sum_{i=1}^{3}b_{i}\hat{e}_i$. The cross product can be writen as 
\begin{equation}
\begin{aligned}
\vec{a}\times\vec{b}
&=\left(\sum_{i=1}^{3}a_i\hat{e}_i\right)\times\left(\sum_{i=1}^{3}b_j\hat{e}_j\right)\\
&=\sum_{i,j=1}^{3}a_ib_j\left(\hat{e}_i\times\hat{e}_j\right)\\
&=\sum_{i,j=1}^{3}a_ib_j\sum_{k=1}^3\varepsilon_{i,j,k}\hat{e}_k,
\end{aligned}
\end{equation}
denoted as 
\begin{equation}
\vec{a}\times\vec{b}=\sum_{i,j,k=1}^{3}a_ib_j\varepsilon_{i,j,k}\hat{e}_k
\quad\text{or}\quad
\left(\vec{a}\times\vec{b}\right)_k=\sum_{i,j=1}^{3}a_ib_j\varepsilon_{i,j,k}.
\end{equation}


\subsection{Vector Triple Product}
For vectors $\vec{a}$, $\vec{b}$ and $\vec{c}$, if we write $\displaystyle \vec{a} = \sum_{i=1}^{3}a_{i}\hat{e}_i$, $\displaystyle \vec{b} = \sum_{i=1}^{3}b_{i}\hat{e}_i$ and $\displaystyle \vec{c} = \sum_{i=1}^{3}c_{i}\hat{e}_i$, the product
\begin{align}
\vec{a}\times\left(\vec{b}\times\vec{c}\right)
&=\sum_{ijk=1}^3\hat{e}_i\left(\vec{a}\times\left(\vec{b}\times\vec{c}\right)\right)_i
\\
&=\sum_{i,j,k=1}^3\hat{e}_i\varepsilon_{i,j,k} a_j  {\color{red}\left(\vec{b}\times\vec{c}\right)_k}
\\
&=\sum_{i,j,k=1}^3\hat{e}_i\varepsilon_{i,j,k} a_j  {\color{red}\sum_{\ell m=1}^3\varepsilon_{k,\ell,m}b_{\ell}c_m}
\\
&=\sum_{i,j,k,\ell,m=1}^3\hat{e}_i\varepsilon_{i,j,k} \varepsilon_{k,\ell,m}a_j  b_{\ell}c_m
\\
&=\sum_{i,j,k,\ell,m=1}^3\hat{e}_i\varepsilon_{k,i,j} \varepsilon_{k,\ell,m}a_j  b_{\ell}c_m
\\
&=\sum_{i,j,\ell,m=1}^3\hat{e}_i\left(\delta_{i\ell}\delta_{jm}-\delta_{im}\delta_{j\ell}\right)a_j  b_{\ell}c_m
\\
&=\sum_{i,j=1}^3\left( a_j  b_i c_j - a_j  b_j c_i\right)\hat{e}_i
\\
&=\left(\sum_{j=1}^3a_jc_j\right)\left(\sum_{i=1}^3\hat{e}_ib_j\right)-
		\left(\sum_{j=1}^3a_jb_j\right)\left(\sum_{i=1}^3\hat{e}_ic_j\right)
\\[6pt]
&=\Big(\vec{a}\cdot\vec{c}\Big)\vec{b}-\left(\vec{a}\cdot\vec{b}\right)\vec{c}
\end{align}

\noindent\fbox{\begin{minipage}{0.99\textwidth}
Using above result, the proof in class can be reduced to 
\begin{align}
\textbf{u}\times\left(\nabla\times\textbf{u}\right)
&= \sum_{i,j=1}^3\left( u_j  \partial_i u_j - u_j  \partial_j u_i\right)\hat{e}_i\\
&= \sum_{i,j=1}^3 \partial_i\hat{e}_i \left(\frac{1}{2} u_j^2\right)
	- \sum_{i,j=1}^3 u_j  \partial_j u_i\hat{e}_i\\
&= \sum_{i=1}^3 \partial_i\hat{e}_i \left(\sum_{j=1}^{3}\frac{1}{2} u_j^2\right)
	- \sum_{j=1}^3 u_j  \partial_j \left(\sum_{i=1}^{3}u_i\hat{e}_i\right)\\
&= \frac{1}{2}\nabla\lVert\textbf{u}\rVert
	- \sum_{j=1}^3 u_j  \partial_j \textbf{u}\\
&= \frac{1}{2}\nabla\lVert\textbf{u}\rVert
	- \left(\textbf{u}\cdot\nabla\right)\textbf{u}.
\end{align}
Last, rearranging the equation, we get $\displaystyle \left(\textbf{u}\cdot\nabla\right)\textbf{u} + \textbf{u}\times\left(\nabla\times\textbf{u}\right) = \frac{1}{2}\nabla\lVert\textbf{u}\rVert$.
\end{minipage}}




%================================================================================================
\end{document}
