### Bernoullis' Theorem

For stationary. isentropic flows and in the absence of external forces,
$$
\textbf{u} \cdot \nabla \left(w + \frac{1}{2}\lVert\textbf{u}\rVert^2\right) = 0
\Leftrightarrow
\frac{d}{dt}\left(\frac{1}{2}\lVert\textbf{u}\rVert^2+w\right)(\textbf{x}(t)) = 0
\label{eq: bernoulli }
$$
which means $\displaystyle \frac{1}{2}\lVert\textbf{u}\rVert^2 + w$ is constant along stream, where $x(t)$ satisfies $\displaystyle \frac{d}{dt}\textbf{x}(t) = \textbf{u}(\textbf{x}(t))$ (Streamline of flow).

> The same result holds if the force $\textbf{b}$ is conservative, i.e. $\textbf{b}=-\nabla \varphi$ for some function $\varphi, w$ replaced by $w+\varphi$ in above statement $(\ref{eq: bernoulli })$.

> Rmk:
>
> Note, if flow is stationary, homogeneous (i.e. $\rho = \rho_0$ is constant in $D$)  and incompressible, the flow is isentropic with $w=p/\rho_0$ hence the statement $(\ref{eq: bernoulli })$ will holds.

#### Proof

By Lemma 1,
$$
\frac{1}{2}\nabla\lVert\textbf{u}\rVert^2 = \left(\textbf{u}\cdot \nabla\right)\textbf{u} + \textbf{u}\times\left(\nabla\times\textbf{u}\right).
$$
Since the flow is steady, we have
$$
\textbf{u}_t + \left(\textbf{u}\cdot \nabla\right) \textbf{u} = -\nabla w
$$
so that 
$$
\nabla w + \left(\textbf{u}\cdot \nabla\right) \textbf{u} = -\textbf{u}_t = 0
\quad\Rightarrow\quad 
\left(\textbf{u}\cdot \nabla\right) \textbf{u} = - \nabla w.
\label{eq: steady flow result }
$$
Consider, 
$$
\nabla\left(\frac{1}{2}\lVert\textbf{u}\rVert^2 + w\right) = \left(\textbf{u}\cdot \nabla\right)\textbf{u} + \textbf{u}\times\left(\nabla\times\textbf{u}\right) + \nabla w
$$
using the result of  $(\ref{eq: steady flow result })$, we have 
$$
\nabla\left(\frac{1}{2}\lVert\textbf{u}\rVert^2 + w\right) = \textbf{u}\times\left(\nabla\times\textbf{u}\right)
$$
so that 
$$
\textbf{u}\cdot\nabla\left(\frac{1}{2}\lVert\textbf{u}\rVert^2 + w\right) = \textbf{u}\cdot\left(\textbf{u}\times\left(\nabla\times\textbf{u}\right)\right) = 0
$$
Taking the divergence, 
$$
\nabla w = -\operatorname{div}\left((\textbf{u}\cdot\nabla)\textbf{u}\right),\quad \text{in $D$.}
$$
By $(\ref{eq: steady flow result })$, $\displaystyle \frac{\partial W}{\partial \textbf{n}}\Bigg|_{\partial D} = \nabla w\cdot \textbf{n} = - (\textbf{u}\cdot\nabla)\textbf{u}\cdot \textbf{n}$, since $w$ satisfies the elliptic PDE with boundary condition, it shows that $w$ is a finction independent of the time $t$:
$$
\frac{d}{dt}\left(\frac{1}{2}\lVert\textbf{u}\rVert^2+w\right)(\textbf{x}(t))
=\textbf{u} \cdot \nabla \left(w + \frac{1}{2}\lVert\textbf{u}\rVert^2\right)(\textbf{x}(t)) 
= 0
$$
or 
$$
\frac{d}{dt}\left(\frac{1}{2}\lVert\textbf{u}\rVert^2+w\right)(\textbf{x}(2)) - \frac{d}{dt}\left(\frac{1}{2}\lVert\textbf{u}\rVert^2+w\right)(\textbf{x}(1)) = \int_{t_1}^{t_2} \left(\frac{1}{2}\lVert\textbf{u}\rVert^2+w\right)dt = 0
$$
 That is $\displaystyle \frac{1}{2}\lVert\textbf{u}\rVert^2+w$ is a constant along stream line.

#### Example

Consider a fluid flow in a channel

<u>FIg</u>

Suppose the pressure is a function of $\textbf{x}$ only and the pressure $p_1$ at $\textbf{x}=0$ is greater than the pressure $p_2$. Then the fluid will flow from left to right with the velocity $\textbf{u}(x,y,t) = (u_1(x,y),0,0)$ and the pressure $\textbf{p}(x,y,t) = p(\textbf{x})$. Suppose the density of fluid $\rho=\rho_0$ is a constant  and the fluid is incompressible.





