### Proposition

For isentropic flow (in the absence of external forces) with $\vec{\xi} = \nabla \times \textbf{u}$ and $\textbf{W} = \vec{\xi} /\rho$ we have
$$
\frac{D\xi}{Dt} - \left(\vec{\xi}\cdot\nabla\right)\textbf{u} + \xi \left(\operatorname{div}\textbf{u}\right) = 0
$$
and
$$
\frac{D\textbf{W} }{Dt} - \left(\textbf{W} \cdot\nabla\right)\textbf{u} = 0
$$
and
$$
w\left(\varphi(\textbf{x},t),t\right) = \nabla \varphi_t(\textbf{x}) \cdot \textbf{W} (\textbf{x})
$$
where $\varphi_t$ is the flow map and $\nabla \varphi_t$  is its Jocobian matrix.

#### Proof $(1)$ 

> **Recall :**
> $$
> \frac{\partial \textbf{u}}{\partial t} + \textbf{u}\cdot\nabla \textbf{u} = -\frac{\nabla p}{\rho} = \nabla w
> $$
> and
> $$
> \frac{1}{2}\left(\lVert\textbf{u}\rVert^2\right) = \textbf{u}\times\left(\nabla\times\textbf{u}\right) + \left(\textbf{u}\cdot\nabla\right)\textbf{u}
> $$

Taking the cross and using the properties $\nabla \times \left(\nabla f\right) = 0$ for any function $f$, we get
$$
\nabla\times\left(
\frac{\partial \textbf{u}}{\partial t} + \frac{1}{2}\nabla\left(\lVert \textbf{u}\rVert^2\right) - \textbf{u}\times\left(\nabla \times \textbf{u}\right)\right) 
= \nabla\times\left(
\nabla w
\right) = 0
$$
then
$$
\nabla \times \frac{\partial \textbf{u}}{\partial t} - \nabla \times\left(\textbf{u}\times \left(\nabla \times\textbf{u}\right)\right)
=
\frac{\partial}{\partial t}\left( \nabla \times \textbf{u}\right) - \nabla \times\left(\textbf{u}\times \left(\nabla \times\textbf{u}\right)\right)
= 0
$$
since $\xi = \nabla \times \textbf{u}$, we get
$$
\frac{\partial \xi}{\partial t} - \nabla \times\left(\textbf{u}\times \xi\right)
= 0
$$

> **Recall : **
> $$
> \begin{aligned}
> \nabla\times\left(\textbf{A}\times \textbf{B}\right) 
> &= \textbf{A} \nabla \cdot \textbf{B} 
> 	- \textbf{B}\nabla\cdot \textbf{A} 
> 	+ \left(\textbf{B}\cdot\nabla\right)\textbf{A}
> 	- \left(\textbf{A}\cdot\nabla\right)\textbf{B}\\
> &= \textbf{A} \operatorname{div} \textbf{B} 
> 	- \textbf{B}\operatorname{div} \textbf{A} 
> 	+ \left(\textbf{B}\cdot\nabla\right)\textbf{A}
> 	- \left(\textbf{A}\cdot\nabla\right)\textbf{B}\\
> \end{aligned}
> $$

Then
$$
\begin{aligned}
0 &= \frac{\partial \xi}{\partial t} - \nabla \times\left(\textbf{u}\times \xi\right)\\
&= \frac{\partial \xi}{\partial t}
- \textbf{u} \operatorname{div} \xi 
	+ \xi \operatorname{div} \textbf{u} 
	- \left(\xi\cdot\nabla\right)\textbf{u}
	+ \left(\textbf{u}\cdot\nabla\right)\xi\\
&= \frac{\partial \xi}{\partial t}
	+ \xi \operatorname{div} \textbf{u} 
	- \left(\xi\cdot\nabla\right)\textbf{u}
	+ \left(\textbf{u}\cdot\nabla\right)\xi
\end{aligned}
$$
or 
$$
\frac{D\xi}{Dt} - \left(\xi\cdot\nabla\right)\textbf{u} + \left(\textbf{u}\cdot\nabla\right)\xi = 0
$$
which satiesfy equation $(1)$. 

#### Proof  $(2)$

$$
\begin{aligned}
\frac{D\textbf{W}}{Dt} 
&= \frac{D}{Dt}\left(\frac{\xi}{\rho}\right)\\
&= \left(\frac{\xi_t}{\rho} - \frac{\xi}{\rho^2}\rho_t\right) 
	+ \left(\frac{\textbf{u}\cdot\nabla \xi}{\rho} 
	- \frac{\xi\left(\textbf{u}\cdot\nabla \rho\right)}{\rho} \right)\\
&= \frac{1}{\rho} \frac{D\xi}{Dt} - \frac{\xi}{\rho^2}\left(\rho_t + \textbf{u}\cdot\nabla\rho\right)\\
&= \frac{1}{\rho} \frac{D\xi}{Dt} - \frac{\xi}{\rho^2}\left(\rho_t + \operatorname{div}(\textbf{u}\rho) - \rho\operatorname{div}\textbf{u} \right)\\
&=\frac{1}{\rho} \frac{D\xi}{Dt} + \frac{\xi}{\rho}\operatorname{div}\textbf{u}\\
&= \frac{1}{\rho}\left(\xi\cdot\nabla\right)\textbf{u} - \frac{\xi}{\rho}\left(\operatorname{div}\textbf{u}\right) + \frac{\xi}{\rho}\left(\operatorname{div}\textbf{u}\right)\\
&= \frac{1}{\rho}\left(\xi\cdot\nabla\right)\textbf{u}
\end{aligned}
$$

which satiesfy equation $(2)$.

#### Proof  $(3)$

Let $F(\textbf{x},t) = w(\varphi(\textbf{x},t),t)$ and $G(\textbf{x},t) = \nabla \varphi_t(\textbf{x})\cdot\textbf{W}(\textbf{x},0)$, by equation $(2)$ 
$$
\frac{\partial F}{\partial t} = \frac{D\textbf{W}}{Dt} = \left(\textbf{W}\cdot\nabla\right)\textbf{u} = \left(F\cdot\nabla\right)\textbf{u}
$$
On the other hand,
$$
\begin{aligned}
\frac{\partial G}{\partial t} 
&= \frac{\partial }{\partial t}\left(\nabla \varphi_t(\textbf{x})\cdot\textbf{W}(\textbf{x},0)\right) \\
&= \nabla \left(\frac{\partial \varphi_t(\textbf{x})}{\partial t}\right) \cdot \textbf{W}(\textbf{x},0)\\
&= \nabla \left(\textbf{u}\left(\varphi(\textbf{x},t),t\right)\right)\cdot\textbf{W}(\textbf{x},0)\\
&= \nabla \textbf{u} \cdot \nabla \varphi_t(\textbf{x}) \cdot \textbf{W}(\textbf{x},0)\\
&= \left(G\cdot\nabla\right)\cdot \textbf{u}
\end{aligned}
$$
Thus $F$ and $G$ satisfies the same ODE system and 
$$
F(\textbf{x},0) = G(\textbf{x},0) = \textbf{W}(\textbf{x},0)
$$

> **Recall :**
>
> The flow map is given by
> $$
> \begin{cases} \displaystyle 
> \frac{\partial}{\partial t} \varphi (\textbf{x},t) = \textbf{u}\left(\varphi(\textbf{x},t),t\right) & t>0\\
> \varphi(\textbf{x},0)=\textbf{x} & x\in D
> \end{cases}
> $$

Hence, by uniqueness of ODE, $F = G$ or $w\left(\varphi(\textbf{x},t),t\right) = \nabla \varphi_t(\textbf{x}) \cdot \textbf{W} (\textbf{x})$

#### Some properties of vortisity

1. If $\xi(\textbf{x},0) = 0$, then $\xi(\textbf{x},t) = 0$ satiesfies $(1)$ if uniqueness applied. Hence the flow that start off irrotational reamin irrotational $\forall t>0$.
    $$
    \frac{D\xi}{Dt} - \left(\xi\cdot\nabla\right)\textbf{u} + \xi \left(\operatorname{div}\textbf{u}\right) = 0
    $$

2. For $2$-dimensional flow $\textbf{u} = (u,v,0)$ and $\xi = (0,0,\xi)$, we have $\xi = \partial_x v - \partial_y u$ and the circulation theroem and Stoke's theorem implies that, if $\Sigma_t = \varphi_t(\Sigma)$ and $\Sigma$ is a region in the fluid and $\varphi_t$ is the flow map, then
    $$
    \int_{\Sigma_t} \xi dA = \int_{\partial \Sigma_t} \textbf{u}\cdot d\textbf{x} = \text{constant}
    $$
    in time. Moreover
    $$
    \left(\textbf{w}\cdot \nabla\right)\textbf{u} = (0,0,\xi/\rho)\cdot \nabla(u,v,0) 
    = (0,0,\xi) \cdot (\partial_x u, \partial_y,0 ) = 0
    $$
    so that, by equation $(2)$
    $$
    \frac{DW}{Dt} = 0
    $$
    then $\xi/\rho$ is a constant $\forall t>0$.

### Definition

A force $\textbf{b}$ in a region is said to be conserve if $\exists$ a function $f$, s.t.
$$
\textbf{b} = -\nabla f
$$
e.g. the gravitaional force $g$ is conservative.

> **Rmk :**
>
> For a fluid with conservative external force and constant 
